hol-light/stateful/holConsistencyScript.sml
@@ -1,5 +1,5 @@
 open HolKernel boolLib bossLib lcsymtacs
-open setSpecTheory holSyntaxTheory holSoundnessTheory
+open setSpecTheory holSyntaxTheory holSyntaxExtraTheory holSemanticsTheory holSoundnessTheory
 val _ = temp_tight_equality()
 val _ = new_theory"holConsistency"
 
@@ -10,22 +10,5 @@ val is_consistent_def = xDefine "is_consistent_def"`
     ∀i. i models (sigof ctxt, set (axexts ctxt)) ⇒
         ∃i'. i' models (thyof ctxt)`
 val _ = Parse.overload_on("is_consistent",``is_consistent0 ^mem``)
-
-(*
-val consistency = store_thm("consistency",
-  ``is_set_theory ^mem ⇒
-    ∀ctxt. context_ok ctxt ∧
-           FILTER (λu. ∃p. u = NewAxiom p) ctxt = [] ⇒
-      (ctxt,[]) |- (Var "x" Bool === Var "x" Bool) ∧
-      ¬((ctxt,[]) |- (Var "x" Bool === Var "y" Bool))``,
-  rw[] >- (
-    match_mp_tac (List.nth(CONJUNCTS proves_rules,8)) >>
-    simp[term_ok_def,type_ok_def] >>
-    imp_res_tac context_ok_sig >>
-    fs[is_std_sig_def] ) >>
-  spose_not_then strip_assume_tac >>
-  imp_res_tac soundness >>
-  fs[entails_def]
-*)
 
 val _ = export_theory()
